prove totality and determinism on tweaked semantics (with cheats)
The cheats are on two lemmas about monotonicity of the FFI state, which
should be easy to push through (since any sequence of call_FFIs should
satisfy them). Hopefully they're not wrong...

semantics/semanticsScript.sml
@@ -33,8 +33,7 @@ val semantics_prog_def = Define `
      FFI, and the accumulated io events match the given io_list *)
   ?k ffi r.
     evaluate_prog_with_clock state k prog = (ffi,r) ∧
-    r ≠ Rerr (Rabort Rtype_error) ∧
-    (r = Rerr (Rabort Rtimeout_error) ⇒ IS_SOME ffi.final_event) ∧
+    (∀a. r = Rerr (Rabort a) ⇒ IS_SOME ffi.final_event) ∧
     (outcome =
      case ffi.final_event of
      | NONE => Success
@@ -56,7 +55,8 @@ val semantics_prog_def = Define `
 (semantics_prog state prog Fail ⇔
   (* there is a clock for which evaluation produces a runtime type error *)
   ∃k ffi.
-    evaluate_prog_with_clock state k prog = (ffi, Rerr (Rabort Rtype_error)))`;
+    evaluate_prog_with_clock state k prog = (ffi, Rerr (Rabort Rtype_error)) ∧
+    ffi.final_event = NONE)`;
 
 val _ = Datatype`semantics = CannotParse | IllTyped | Execute (behaviour set)`;
 
