semantics/proofs/semanticsPropsScript.sml
@@ -12,22 +12,58 @@ val evaluate_prog_io_events_mono = Q.store_thm("evaluate_prog_io_events_mono",
   `∀k1 k2 s e p.
     k1 ≤ k2 ⇒
     (FST (evaluate_prog (s with clock := k1) e p)).ffi.io_events ≼
-    (FST (evaluate_prog (s with clock := k2) e p)).ffi.io_events`,
+    (FST (evaluate_prog (s with clock := k2) e p)).ffi.io_events ∧
+    (IS_SOME (FST (evaluate_prog (s with clock := k1) e p)).ffi.final_event ⇒
+      (FST (evaluate_prog (s with clock := k1) e p)).ffi.io_events =
+      (FST (evaluate_prog (s with clock := k2) e p)).ffi.io_events)`,
   cheat)
+
+val evaluate_prog_final_event_mono = Q.store_thm("evaluate_prog_final_event_mono",
+  `k1 ≤ k2 ⇒
+   IS_SOME(FST(evaluate_prog (s with clock := k1) e p)).ffi.final_event ⇒
+   (FST(evaluate_prog (s with clock := k2) e p)).ffi.final_event =
+     SOME(THE(FST(evaluate_prog (s with clock := k1) e p)).ffi.final_event)`,
+  cheat)
+
+local
+  open bigStepTheory
+  open semanticPrimitivesTheory
+in
+val prog_add_to_counter = Q.store_thm("prog_add_to_counter",
+  `∀ck env st prog res.
+      evaluate_prog ck env st prog res ⇒
+     ∀r2 r3 extra.
+       res = (r2,r3) ∧ ck ∧ (SND r3 ≠ Rerr (Rabort Rtimeout_error)) ⇒
+         evaluate_prog T env (st with clock := st.clock + extra) prog (r2 with clock := r2.clock + extra,r3)`,
+  ho_match_mp_tac evaluate_prog_ind >> rw[] >>
+  rw[Once evaluate_prog_cases] >>
+  imp_res_tac top_add_to_counter >>
+  fs[] >> rw[] >> fs[] >>
+  `r ≠ Rerr (Rabort Rtimeout_error)`
+    by (Cases_on`r` >> fs[combine_mod_result_def]) >>
+  fs[] >> metis_tac[])
+end
+
 (* -- *)
 
 val semantics_prog_total = Q.store_thm("semantics_prog_total",
   `∀s p. ∃b. semantics_prog s p b`,
   rw[] >>
-  Cases_on`∃k ffi. evaluate_prog_with_clock s k p = (ffi,Rerr (Rabort Rtype_error))`
+  Cases_on`∃k ffi. evaluate_prog_with_clock s k p = (ffi,Rerr (Rabort Rtype_error)) ∧ ffi.final_event = NONE`
   >- metis_tac[semantics_prog_def] >> fs[] >>
   Cases_on`∃k ffi r.
     evaluate_prog_with_clock s k p = (ffi,r) ∧
-    (r = Rerr (Rabort Rtimeout_error) ⇒ IS_SOME ffi.final_event)`
+    (∀a. r = Rerr (Rabort a) ⇒ IS_SOME ffi.final_event)`
   >- metis_tac[semantics_prog_def] >> fs[] >>
   qexists_tac`Diverge (build_lprefix_lub (IMAGE (λk. fromList (FST (evaluate_prog_with_clock s k p)).io_events) UNIV))` >>
   simp[semantics_prog_def] >>
-  conj_tac >- metis_tac[PAIR] >>
+  conj_tac >- (
+    strip_tac >>
+    rpt(first_x_assum(qspec_then`k`mp_tac)) >>
+    Cases_on`evaluate_prog_with_clock s k p`>>simp[]>>
+    Cases_on`r`>>simp[]>>
+    Cases_on`e`>>simp[]>>
+    Cases_on`a`>>simp[]) >>
   match_mp_tac build_lprefix_lub_thm >>
   qho_match_abbrev_tac`lprefix_chain (IMAGE (λk. fromList (g k)) UNIV)` >>
   ONCE_REWRITE_TAC[GSYM o_DEF] >>
@@ -49,57 +85,94 @@ val prog_clocked_zero_determ = Q.prove(
   discharge_hyps >- (simp[] >> metis_tac[]) >>
   metis_tac[prog_determ,PAIR_EQ])
 
-(*
+val prog_clocked_timeout_smaller = Q.prove(
+  `evaluate_prog T x (y with clock := a) z (p,q,r) ∧
+   evaluate_prog T x (y with clock := b) z (t,u,Rerr (Rabort Rtimeout_error)) ∧
+   r ≠ Rerr (Rabort	Rtimeout_error)
+   ⇒
+   b < a`,
+  rpt strip_tac >>
+  CCONTR_TAC >> fs[NOT_LESS] >>
+  fs[LESS_EQ_EXISTS] >>
+  imp_res_tac prog_add_to_counter >> rfs[] >>
+  rw[] >>
+  metis_tac[prog_determ,PAIR_EQ])
+
+val with_clock_ffi = Q.prove(
+  `(s with clock := x).ffi = s.ffi`,EVAL_TAC)
+
+val tac0 =
+    fs[evaluate_prog_with_clock_def,LET_THM] >>
+    first_assum(split_applied_pair_tac o lhs o concl) >> fs[] >> rpt var_eq_tac >>
+    first_assum(split_applied_pair_tac o lhs o concl) >> fs[] >> rpt var_eq_tac >>
+    imp_res_tac functional_evaluate_prog >>
+    fs[bigStepTheory.evaluate_whole_prog_def]
+
+val tac =
+    tac0 >>
+    Cases_on`∃a. r = Rerr (Rabort a)` >> fs[] >- (
+      fs[] >>
+      qmatch_assum_abbrev_tac`if X then Y else Z` >>
+      reverse(Cases_on`X`)>>fs[Abbr`Y`,Abbr`Z`] >- (
+        rw[] >> rfs[] >> fs[]) >>
+      Cases_on`a` >- (
+        imp_res_tac prog_clocked_min_counter >> fs[] >>
+        `st''.ffi = st'.ffi` by (
+          metis_tac[prog_clocked_zero_determ,SND,
+                    semanticPrimitivesTheory.result_11,
+                    semanticPrimitivesTheory.error_result_11,
+                    semanticPrimitivesTheory.abort_distinct,
+                    with_clock_ffi,
+                    semanticPrimitivesTheory.state_component_equality] ) >>
+          fs[IS_SOME_EXISTS] >> fs[] ) >>
+      imp_res_tac prog_clocked_timeout_smaller >> fs[] >>
+      imp_res_tac LESS_IMP_LESS_OR_EQ >>
+      imp_res_tac evaluate_prog_final_event_mono >>
+      fs[IS_SOME_EXISTS,PULL_EXISTS] >>
+      metis_tac[FST,NOT_SOME_NONE] ) >>
+    every_case_tac >> fs[] >>
+    imp_res_tac prog_clocked_min_counter >> fs[] >>
+    imp_res_tac prog_clocked_zero_determ >> rfs[]
+
+val tac1 =
+    metis_tac[semanticPrimitivesTheory.result_11,
+              semanticPrimitivesTheory.error_result_11,
+              semanticPrimitivesTheory.abort_distinct,
+              PAIR_EQ,IS_SOME_EXISTS,NOT_SOME_NONE]
+
 val semantics_prog_deterministic = Q.store_thm("semantics_prog_deterministic",
   `∀s p b b'. semantics_prog s p b ∧
               semantics_prog s p b' ⇒
               b = b'`,
   ntac 2 gen_tac >> reverse Cases >> rw[semantics_prog_def] >- (
-    Cases_on`b'`>>fs[semantics_prog_def] >-
-      metis_tac[semanticPrimitivesTheory.result_11,
-                semanticPrimitivesTheory.error_result_11,
-                semanticPrimitivesTheory.abort_distinct,
-                PAIR_EQ] >>
-    fs[evaluate_prog_with_clock_def,LET_THM] >>
-    first_assum(split_applied_pair_tac o lhs o concl) >> fs[] >> rw[] >>
-    first_assum(split_applied_pair_tac o lhs o concl) >> fs[] >> rw[] >>
-    imp_res_tac functional_evaluate_prog >>
-    fs[bigStepTheory.evaluate_whole_prog_def] >>
-    every_case_tac >> fs[] >>
-    imp_res_tac prog_clocked_min_counter >> fs[] >>
-    imp_res_tac prog_clocked_zero_determ >> rfs[] )
+    Cases_on`b'`>>fs[semantics_prog_def] >- tac1 >> tac)
   >- (
     Cases_on`b'`>>fs[semantics_prog_def]
-    >- metis_tac[semanticPrimitivesTheory.result_11,
-                 semanticPrimitivesTheory.error_result_11,
-                 semanticPrimitivesTheory.abort_distinct,
-                 PAIR_EQ]
+    >- tac1
     >- (
-      fs[evaluate_prog_with_clock_def,LET_THM] >>
-      first_assum(split_applied_pair_tac o lhs o concl) >> fs[] >> rpt var_eq_tac >>
-      first_assum(split_applied_pair_tac o lhs o concl) >> fs[] >> rpt var_eq_tac >>
-      imp_res_tac functional_evaluate_prog >>
-      fs[bigStepTheory.evaluate_whole_prog_def] >>
-      pop_assum mp_tac >> IF_CASES_TAC >> fs[] >> strip_tac >>
+      tac0 >>
+      qmatch_assum_abbrev_tac`if X then Y else Z` >>
+      reverse(Cases_on`X`)>>fs[Abbr`Y`,Abbr`Z`] >- (
+        rw[] >> rfs[] >> fs[]) >>
+      Cases_on`∃a a'. r = Rerr (Rabort a) ∧ r' = Rerr (Rabort a')` >> fs[] >- (
+        metis_tac[LESS_EQ_CASES,
+                  evaluate_prog_final_event_mono,
+                  evaluate_prog_io_events_mono,
+                  FST,THE_DEF,IS_SOME_EXISTS] ) >>
+      Cases_on`r = Rerr (Rabort Rtimeout_error) ∨ r' = Rerr (Rabort Rtimeout_error)` >- (
+        metis_tac[prog_clocked_timeout_smaller,
+                  LESS_IMP_LESS_OR_EQ,
+                  evaluate_prog_io_events_mono,
+                  evaluate_prog_final_event_mono,
+                  FST,THE_DEF,IS_SOME_EXISTS] ) >>
       imp_res_tac prog_clocked_min_counter >> fs[] >>
-      imp_res_tac prog_clocked_zero_determ >>
-      rfs[semanticPrimitivesTheory.state_component_equality] )
-    >- (
-      fs[evaluate_prog_with_clock_def,LET_THM] >>
-      first_assum(split_applied_pair_tac o lhs o concl) >> fs[] >> rpt var_eq_tac >>
-      first_assum(split_applied_pair_tac o lhs o concl) >> fs[] >> rpt var_eq_tac >>
-      imp_res_tac functional_evaluate_prog >>
-      fs[bigStepTheory.evaluate_whole_prog_def] >>
-      every_case_tac >> fs[] >>
-      imp_res_tac prog_clocked_min_counter >> fs[] >>
-      imp_res_tac prog_clocked_zero_determ >> rfs[] ))
+      first_x_assum(mp_tac o MATCH_MP (REWRITE_RULE[GSYM AND_IMP_INTRO](GEN_ALL prog_clocked_zero_determ))) >>
+      disch_then(fn th => first_x_assum(mp_tac o MATCH_MP th)) >>
+      simp[semanticPrimitivesTheory.state_component_equality])
+    >- tac)
   >- (
     Cases_on`b'`>>fs[semantics_prog_def]
     >- metis_tac[unique_lprefix_lub] >>
-    metis_tac[semanticPrimitivesTheory.result_11,
-              semanticPrimitivesTheory.error_result_11,
-              semanticPrimitivesTheory.abort_distinct,
-              PAIR_EQ]))
-*)
+    tac1))
 
 val _ = export_theory()
